theories/tests/lock.v
@@ -1,0 +1,3 @@
+Require Import iris_os.clang.logic.
+
+(* Spin lock *)
